Wavelet/Semantics/Guard.lean
@@ -1,99 +1,62 @@
 import Wavelet.Semantics.Defs
 
-/-! Definitions to guard a semantics with a given state or label invariant. -/
+/-! Definitions to guard a semantics with a given label restriction. -/
 
 namespace Wavelet.Semantics
 
-/-- Restricts an LTS by imposing a state invariant. -/
-inductive Lts.GuardState {S} (Inv : S → Prop) (lts : Lts S E) : Lts S E where
-  | step : Inv s → Inv s' → lts.Step s e s' → GuardState Inv lts s e s'
-
-/-- Guards the transition of a semantics with the given invariant. -/
-def guardState
-  [Arity Op]
-  (sem : Semantics Op V m n)
-  (Inv : sem.S → Prop) :
-  Semantics Op V m n :=
-  {
-    S := sem.S,
-    init := sem.init,
-    lts := sem.lts.GuardState Inv,
-  }
-
 /-- Modifies labels with a relation. -/
-inductive Lts.GuardLabel {S} (Guard : E → E' → Prop) (lts : Lts S E) : Lts S E' where
-  | step : Guard e e' → lts.Step s e s' → GuardLabel Guard lts s e' s'
+inductive Lts.Guard {S} (P : E → E' → Prop) (lts : Lts S E) : Lts S E' where
+  | step : P e e' → lts.Step s e s' → Guard P lts s e' s'
 
 /-- Guards and interprets the labels as another set of operators. -/
-def guardLabel
+def guard
   [Arity Op] [Arity Op']
-  (sem : Semantics Op V m n)
-  (Guard : Label Op V m n → Label Op' V' m' n' → Prop) :
+  (P : Label Op V m n → Label Op' V' m' n' → Prop)
+  (sem : Semantics Op V m n) :
   Semantics Op' V' m' n' := {
     S := sem.S,
     init := sem.init,
-    lts := sem.lts.GuardLabel Guard,
+    lts := sem.lts.Guard P,
   }
 
-/-- Combines `GuardState` and `GuardLabel`. -/
-def Lts.Guard {S}
-  (lts : Lts S E)
-  (Inv : S → Prop)
-  (Guard : E → E' → Prop) : Lts S E' :=
-  (lts.GuardState Inv).GuardLabel Guard
-
-/-- Combines `guardState` and `guardLabel`. -/
-def guard
-  [Arity Op] [Arity Op']
-  (sem : Semantics Op V m n)
-  (Inv : sem.S → Prop)
-  (Guard : Label Op V m n → Label Op' V' m' n' → Prop) :
-  Semantics Op' V' m' n' :=
-  (sem.guardState Inv).guardLabel Guard
-
 /-- Some well-formedness constraints on label guards. -/
-class LawfulLabelGuard [Arity Op] [Arity Op']
+class LawfulGuard [Arity Op] [Arity Op']
   (Guard : Label Op V m n → Label Op' V' m' n' → Prop) where
-  label_guard_tau : Guard .τ .τ
-  label_guard_tau_only : ∀ {l}, Guard .τ l → l.isSilent
-  label_guard_input : ∀ {vals l}, Guard (.input vals) l → l.isSilent ∨ l.isInput
-  label_guard_output : ∀ {vals l}, Guard (.output vals) l → l.isSilent ∨ l.isOutput
-  label_guard_yield : ∀ {op inputs outputs l}, Guard (.yield op inputs outputs) l → l.isSilent ∨ l.isYield
+  guard_tau : Guard .τ .τ
+  guard_tau_only : ∀ {l}, Guard .τ l → l.isSilent
+  guard_input : ∀ {vals l}, Guard (.input vals) l → l.isSilent ∨ l.isInput
+  guard_output : ∀ {vals l}, Guard (.output vals) l → l.isSilent ∨ l.isOutput
+  guard_yield : ∀ {op inputs outputs l}, Guard (.yield op inputs outputs) l → l.isSilent ∨ l.isYield
 
 /-- Introduces a `Guard` step from a single step in the base LTS. -/
 theorem guard_single
   {S : Type u}
   {lts : Lts S E}
-  {Inv : S → Prop}
-  {Guard : E → E' → Prop}
+  {P : E → E' → Prop}
   {s s' : S}
-  (hstep : lts.Step s e s')
-  (hinv₁ : Inv s)
-  (hinv₂ : Inv s')
-  (hinterp : Guard e e') :
-  (lts.Guard Inv Guard).Step s e' s'
-:= by
-  apply Lts.GuardLabel.step hinterp
-  apply Lts.GuardState.step hinv₁ hinv₂ hstep
+  (hguard : P e e')
+  (hstep : lts.Step s e s') :
+  (lts.Guard P).Step s e' s'
+:= Lts.Guard.step hguard hstep
 
-/-- `guardLabel` preserves IO-restricted simulation. -/
-theorem sim_guard_label
+/-- `guard` preserves IO-restricted simulation. -/
+theorem sim_guard
   [Arity Op] [Arity Op']
   [DecidableEq χ]
   [DecidableEq χ']
   [InterpConsts V]
   [InterpConsts V']
   {sem₁ sem₂ : Semantics Op V m n}
-  {Guard : Label Op V m n → Label Op' V' m' n' → Prop}
-  [hguard : LawfulLabelGuard Guard]
+  {P : Label Op V m n → Label Op' V' m' n' → Prop}
+  [hguard : LawfulGuard P]
   (hsim : sem₁ ≲ᵣ sem₂) :
-  sem₁.guardLabel Guard ≲ᵣ sem₂.guardLabel Guard
+  sem₁.guard P ≲ᵣ sem₂.guard P
   := by
   apply Lts.Similarity.intro hsim.Sim
   constructor
   · exact hsim.sim_init
   · intros s₁ s₂ l s₁' hR hstep
-    simp [Semantics.guardLabel] at hstep
+    simp [Semantics.guard] at hstep
     cases hstep with | step hlabel hstep =>
     rename Label Op V m n => l'
     have ⟨s₂', hstep_s₂, hR₂⟩ := hsim.sim_step _ _ _ _ hR hstep
@@ -101,28 +64,28 @@ theorem sim_guard_label
     constructor
     · cases hstep_s₂ with
       | step_yield hstep_yield_s₂ =>
-        replace hstep_yield_s₂ := Lts.GuardLabel.step hlabel hstep_yield_s₂
-        cases hguard.label_guard_yield hlabel <;>
+        replace hstep_yield_s₂ := Lts.Guard.step hlabel hstep_yield_s₂
+        cases hguard.guard_yield hlabel <;>
           rename_i h₁ <;> cases l <;> simp at h₁
         · exact .step_tau (.single hstep_yield_s₂)
         · exact .step_yield hstep_yield_s₂
       | step_input hstep_input_s₂ hstep_tau =>
-        replace hstep_input_s₂ := Lts.GuardLabel.step hlabel hstep_input_s₂
-        replace hstep_tau := hstep_tau.map (Lts.GuardLabel.step hguard.label_guard_tau)
-        cases hguard.label_guard_input hlabel <;>
+        replace hstep_input_s₂ := Lts.Guard.step hlabel hstep_input_s₂
+        replace hstep_tau := hstep_tau.map (Lts.Guard.step hguard.guard_tau)
+        cases hguard.guard_input hlabel <;>
           rename_i h₁ <;> cases l <;> simp at h₁
         · exact .step_tau (hstep_tau.prepend hstep_input_s₂)
         · exact .step_input hstep_input_s₂ hstep_tau
       | step_output hstep_tau hstep_output_s₂ =>
-        replace hstep_output_s₂ := Lts.GuardLabel.step hlabel hstep_output_s₂
-        replace hstep_tau := hstep_tau.map (Lts.GuardLabel.step hguard.label_guard_tau)
-        cases hguard.label_guard_output hlabel <;>
+        replace hstep_output_s₂ := Lts.Guard.step hlabel hstep_output_s₂
+        replace hstep_tau := hstep_tau.map (Lts.Guard.step hguard.guard_tau)
+        cases hguard.guard_output hlabel <;>
           rename_i h₁ <;> cases l <;> simp at h₁
         · exact .step_tau (hstep_tau.tail hstep_output_s₂)
         · exact .step_output hstep_tau hstep_output_s₂
       | step_tau hstep_tau_s₂ =>
-        replace hstep_tau_s₂ := hstep_tau_s₂.map (Lts.GuardLabel.step hguard.label_guard_tau)
-        have := hguard.label_guard_tau_only hlabel
+        replace hstep_tau_s₂ := hstep_tau_s₂.map (Lts.Guard.step hguard.guard_tau)
+        have := hguard.guard_tau_only hlabel
         cases l <;> simp at this
         exact .step_tau hstep_tau_s₂
     · exact hR₂
